theories/Symbolic/PartialEvaluation.v
@@ -28,6 +28,7 @@
 (******************************************************************************)
 
 From Coq Require Import
+     Logic.Eqdep_dec
      Arith.PeanoNat
      Bool.Bool
      Classes.Morphisms
@@ -400,8 +401,16 @@ Module Type PartialEvaluationOn
     | t                               => term_unop uop.not t.
 
     Definition peval_unop' {σ1 σ2} (op : UnOp σ1 σ2) (t : Term Σ σ1) : Term Σ σ2 :=
-      match term_get_val t with
-      | Some v => term_val σ2 (uop.eval op v)
+      match term_get_relval t with
+      | Some v =>
+          match v with
+          | ty.SyncVal _ v => match t with
+                              | term_val _ _ => term_val σ2 (uop.eval op v)
+                              | term_relval _ _ => term_relval σ2 (ty.SyncVal σ2  (uop.eval op v))
+                              | _ => term_unop op t
+                              end
+          | ty.NonSyncVal _ v1 v2 => term_relval σ2 (ty.NonSyncVal _ (uop.eval op v1) (uop.eval op v2))
+          end
       | None   => term_unop op t
       end.
 
@@ -415,9 +424,19 @@ Module Type PartialEvaluationOn
       peval_not t ≡ term_unop uop.not t.
     Proof. funelim (peval_not t); lsolve; now apply proper_term_binop. Qed.
 
+    (* TODO: Problems arise when applying a unop to term_relval (ty.SyncVal _ v), because this becomes a term_val (uop.eval op v) at the end. *)
     Lemma peval_unop'_sound {σ1 σ2} (op : UnOp σ1 σ2) (t : Term Σ σ1) :
       peval_unop' op t ≡ term_unop op t.
-    Proof. unfold peval_unop'; destruct (term_get_val_spec t); subst; easy. Qed.
+    Proof. unfold peval_unop'; destruct (term_get_relval_spec t); subst; try easy.
+           destruct a.
+           - destruct t; cbn; inversion H; try reflexivity; try congruence.
+             { rewrite H0.
+             easy. }
+             inversion H0.
+             apply (inj_pair2_eq_dec _ ty.Ty_eq_dec) in H2.
+             subst; easy.
+           - subst; easy.
+    Qed.
 
     Lemma peval_unop_sound {σ1 σ2} (op : UnOp σ1 σ2) (t : Term Σ σ1) :
       peval_unop op t ≡ term_unop op t.
