theories/Base.v
@@ -73,147 +73,153 @@ Module Type BaseMixin (Import TY : Types).
   Notation CStoreRel := (@NamedEnv PVar Ty RelVal).
   Notation CStore := (@NamedEnv PVar Ty Val).
 
-  (* Definition SMatchResult {N σ} (pat : @Pattern N σ) (Σ : LCtx) : Type := *)
-  (*   { pc : PatternCase pat & NamedEnv (Term Σ) (PatternCaseCtx pc) }. *)
+  Fixpoint mapSyncValNamedEnv {X Σ} (ı : NamedEnv (X := X) Val Σ) : NamedEnv (X := X) RelVal Σ :=
+    match ı with
+    | env.nil => env.nil
+    | env.snoc E db v => env.snoc (mapSyncValNamedEnv E) db (ty.SyncVal (type db) v)
+    end.
 
-  (* Section PatternMatching. *)
-  (*   Context {N : Set}. *)
+  Definition SMatchResult {N σ} (pat : @Pattern N σ) (Σ : LCtx) : Type :=
+    { pc : PatternCase pat & NamedEnv (Term Σ) (PatternCaseCtx pc) }.
 
-  (*   (* Lemma inst_tuple_pattern_match {Σ : LCtx} {σs : Ctx Ty} {Δ : NCtx N Ty} *) *)
-  (*   (*   (ι : Valuation Σ) (p : TuplePat σs Δ) (ts : Env (Term Σ) σs) : *) *)
-  (*   (*   inst (tuple_pattern_match_env p ts) ι = *) *)
-  (*   (*   tuple_pattern_match_env p (inst (T := fun Σ => Env (Term Σ) σs) ts ι). *) *)
-  (*   (* Proof. *) *)
-  (*   (*   unfold inst at 1; cbn. *) *)
-  (*   (*   induction p; cbn. *) *)
-  (*   (*   - reflexivity. *) *)
-  (*   (*   - destruct (env.view ts); cbn. *) *)
-  (*   (*     f_equal. apply IHp. *) *)
-  (*   (* Qed. *) *)
+  Section PatternMatching.
+    Context {N : Set}.
 
-  (*   (* Lemma inst_tuple_pattern_match_reverse {Σ : LCtx} {σs : Ctx Ty} {Δ : NCtx N Ty} *) *)
-  (*   (*   (ι : Valuation Σ) (p : TuplePat σs Δ) (ts : NamedEnv (Term Σ) Δ) : *) *)
-  (*   (*   inst (tuple_pattern_match_env_reverse p ts) ι = *) *)
-  (*   (*   tuple_pattern_match_env_reverse p (inst (T := fun Σ => NamedEnv (Term Σ) Δ) ts ι). *) *)
-  (*   (* Proof. *) *)
-  (*   (*   unfold inst at 1; cbn. *) *)
-  (*   (*   induction p; cbn. *) *)
-  (*   (*   - reflexivity. *) *)
-  (*   (*   - destruct (env.view ts); cbn. *) *)
-  (*   (*     f_equal. apply IHp. *) *)
-  (*   (* Qed. *) *)
+    (* Lemma inst_tuple_pattern_match {Σ : LCtx} {σs : Ctx Ty} {Δ : NCtx N Ty} *)
+    (*   (ι : Valuation Σ) (p : TuplePat σs Δ) (ts : Env (Term Σ) σs) : *)
+    (*   inst (tuple_pattern_match_env p ts) ι = *)
+    (*   tuple_pattern_match_env p (inst (T := fun Σ => Env (Term Σ) σs) ts ι). *)
+    (* Proof. *)
+    (*   unfold inst at 1; cbn. *)
+    (*   induction p; cbn. *)
+    (*   - reflexivity. *)
+    (*   - destruct (env.view ts); cbn. *)
+    (*     f_equal. apply IHp. *)
+    (* Qed. *)
 
-  (*   (* Lemma inst_record_pattern_match {Δ__R : NCtx recordf Ty} {Σ : LCtx} {Δ : NCtx N Ty} *) *)
-  (*   (*   (ι : Valuation Σ) (p : RecordPat Δ__R Δ) (ts : NamedEnv (Term Σ) Δ__R) : *) *)
-  (*   (*   inst (T := fun Σ => NamedEnv (Term Σ) Δ) (record_pattern_match_env p ts) ι = *) *)
-  (*   (*   record_pattern_match_env p (inst ts ι). *) *)
-  (*   (* Proof. *) *)
-  (*   (*   unfold inst at 1; cbn. *) *)
-  (*   (*   induction p; cbn. *) *)
-  (*   (*   - reflexivity. *) *)
-  (*   (*   - destruct (env.view ts); cbn. *) *)
-  (*   (*     f_equal. apply IHp. *) *)
-  (*   (* Qed. *) *)
+    (* Lemma inst_tuple_pattern_match_reverse {Σ : LCtx} {σs : Ctx Ty} {Δ : NCtx N Ty} *)
+    (*   (ι : Valuation Σ) (p : TuplePat σs Δ) (ts : NamedEnv (Term Σ) Δ) : *)
+    (*   inst (tuple_pattern_match_env_reverse p ts) ι = *)
+    (*   tuple_pattern_match_env_reverse p (inst (T := fun Σ => NamedEnv (Term Σ) Δ) ts ι). *)
+    (* Proof. *)
+    (*   unfold inst at 1; cbn. *)
+    (*   induction p; cbn. *)
+    (*   - reflexivity. *)
+    (*   - destruct (env.view ts); cbn. *)
+    (*     f_equal. apply IHp. *)
+    (* Qed. *)
 
-  (*   (* Lemma inst_record_pattern_match_reverse {Δ__R : NCtx recordf Ty} {Σ : LCtx} {Δ : NCtx N Ty} *) *)
-  (*   (*   (ι : Valuation Σ) (p : RecordPat Δ__R Δ) (ts : NamedEnv (Term Σ) Δ) : *) *)
-  (*   (*   inst (record_pattern_match_env_reverse p ts) ι = *) *)
-  (*   (*   record_pattern_match_env_reverse p (inst (T := fun Σ => NamedEnv (Term Σ) Δ) ts ι). *) *)
-  (*   (* Proof. *) *)
-  (*   (*   unfold inst at 1; cbn. *) *)
-  (*   (*   induction p; cbn. *) *)
-  (*   (*   - reflexivity. *) *)
-  (*   (*   - destruct (env.view ts); cbn. *) *)
-  (*   (*     f_equal. apply IHp. *) *)
-  (*   (* Qed. *) *)
+    (* Lemma inst_record_pattern_match {Δ__R : NCtx recordf Ty} {Σ : LCtx} {Δ : NCtx N Ty} *)
+    (*   (ι : Valuation Σ) (p : RecordPat Δ__R Δ) (ts : NamedEnv (Term Σ) Δ__R) : *)
+    (*   inst (T := fun Σ => NamedEnv (Term Σ) Δ) (record_pattern_match_env p ts) ι = *)
+    (*   record_pattern_match_env p (inst ts ι). *)
+    (* Proof. *)
+    (*   unfold inst at 1; cbn. *)
+    (*   induction p; cbn. *)
+    (*   - reflexivity. *)
+    (*   - destruct (env.view ts); cbn. *)
+    (*     f_equal. apply IHp. *)
+    (* Qed. *)
 
-  (*   Definition pattern_match_term_reverse {Σ σ} (pat : @Pattern N σ) : *)
-  (*     forall (pc : PatternCase pat), NamedEnv (Term Σ) (PatternCaseCtx pc) -> Term Σ σ := *)
-  (*     match pat with *)
-  (*     | pat_var x => *)
-  (*         fun _ ts => env.head ts *)
-  (*     | pat_bool => *)
-  (*         fun b _ => term_val ty.bool b *)
-  (*     | pat_list σ x y => *)
-  (*         fun b => *)
-  (*           match b with *)
-  (*           | true => fun _ => term_val (ty.list σ) nil *)
-  (*           | false => fun Eht => *)
-  (*                        let (Eh,t) := env.view Eht in *)
-  (*                        let (E,h)  := env.view Eh in *)
-  (*                        term_binop bop.cons h t *)
-  (*           end *)
-  (*     | pat_pair x y => *)
-  (*         fun _ Exy => *)
-  (*           let (Ex,vτ) := env.view Exy in *)
-  (*           let (E,vσ)  := env.view Ex in *)
-  (*           term_binop bop.pair vσ vτ *)
-  (*     | pat_sum σ0 τ x y => *)
-  (*         fun b => *)
-  (*           match b with *)
-  (*           | true => fun ts => term_unop uop.inl (env.head ts) *)
-  (*           | false => fun ts => term_unop uop.inr (env.head ts) *)
-  (*           end *)
-  (*     | pat_unit => *)
-  (*         fun pc _ => term_val ty.unit pc *)
-  (*     (* | pat_enum E => *) *)
-  (*     (*     fun v _ => term_val (ty.enum E) v *) *)
-  (*     | pat_bvec_split m n x y => *)
-  (*         fun _ Exy => *)
-  (*           let (Ex,vr) := env.view Exy in *)
-  (*           let (E,vl)  := env.view Ex in *)
-  (*           term_binop bop.bvapp vl vr *)
-  (*     | pat_bvec_exhaustive m => *)
-  (*         fun v _ => term_val (ty.bvec m) v *)
-  (*     (* | pat_tuple p => *) *)
-  (*     (*     fun _ ts => term_tuple (tuple_pattern_match_env_reverse p ts) *) *)
-  (*     (* | pat_record R Δ p => *) *)
-  (*     (*     fun _ ts => term_record R (record_pattern_match_env_reverse p ts) *) *)
-  (*     (* | pat_union U x => *) *)
-  (*     (*     fun '(existT K pc) ts => term_union U K (pattern_match_term_reverse (x K) pc ts) *) *)
-  (*     end. *)
+    (* Lemma inst_record_pattern_match_reverse {Δ__R : NCtx recordf Ty} {Σ : LCtx} {Δ : NCtx N Ty} *)
+    (*   (ι : Valuation Σ) (p : RecordPat Δ__R Δ) (ts : NamedEnv (Term Σ) Δ) : *)
+    (*   inst (record_pattern_match_env_reverse p ts) ι = *)
+    (*   record_pattern_match_env_reverse p (inst (T := fun Σ => NamedEnv (Term Σ) Δ) ts ι). *)
+    (* Proof. *)
+    (*   unfold inst at 1; cbn. *)
+    (*   induction p; cbn. *)
+    (*   - reflexivity. *)
+    (*   - destruct (env.view ts); cbn. *)
+    (*     f_equal. apply IHp. *)
+    (* Qed. *)
 
-  (*   Lemma inst_pattern_match_term_reverse {Σ σ} (ι : Valuation Σ) (pat : @Pattern N σ) : *)
-  (*     forall (pc : PatternCase pat) (ts : NamedEnv (Term Σ) (PatternCaseCtx pc)), *)
-  (*       inst (pattern_match_term_reverse pat pc ts) ι = *)
-  (*       pattern_match_val_reverse pat pc (inst (T := fun Σ => NamedEnv (Term Σ) _) ts ι). *)
-  (*   Proof. *)
-  (*     induction pat; cbn. *)
-  (*     - intros _ ts. now env.destroy ts. *)
-  (*     - reflexivity. *)
-  (*     - intros [] ts. *)
-  (*       + reflexivity. *)
-  (*       + now env.destroy ts. *)
-  (*     - intros _ ts. now env.destroy ts. *)
-  (*     - intros [] ts; now env.destroy ts. *)
-  (*     - intros [] ts. reflexivity. *)
-  (*     - reflexivity. *)
-  (*     - intros _ ts. now env.destroy ts. *)
-  (*     - reflexivity. *)
-  (*     - intros _ ts. *)
-  (*       now rewrite <- inst_tuple_pattern_match_reverse. *)
-  (*     - intros _ ts. f_equal. *)
-  (*       apply inst_record_pattern_match_reverse. *)
-  (*     - intros [] ts. cbn. f_equal. f_equal. apply H. *)
-  (*   Qed. *)
+    Definition pattern_match_term_reverse {Σ σ} (pat : @Pattern N σ) :
+      forall (pc : PatternCase pat), NamedEnv (Term Σ) (PatternCaseCtx pc) -> Term Σ σ :=
+      match pat with
+      | pat_var x =>
+          fun _ ts => env.head ts
+      | pat_bool =>
+          fun b _ => term_val ty.bool b
+      (* | pat_list σ x y => *)
+      (*     fun b => *)
+      (*       match b with *)
+      (*       | true => fun _ => term_val (ty.list σ) nil *)
+      (*       | false => fun Eht => *)
+      (*                    let (Eh,t) := env.view Eht in *)
+      (*                    let (E,h)  := env.view Eh in *)
+      (*                    term_binop bop.cons h t *)
+      (*       end *)
+      | pat_pair x y =>
+          fun _ Exy =>
+            let (Ex,vτ) := env.view Exy in
+            let (E,vσ)  := env.view Ex in
+            term_binop bop.pair vσ vτ
+      (* | pat_sum σ0 τ x y => *)
+      (*     fun b => *)
+      (*       match b with *)
+      (*       | true => fun ts => term_unop uop.inl (env.head ts) *)
+      (*       | false => fun ts => term_unop uop.inr (env.head ts) *)
+      (*       end *)
+      | pat_unit =>
+          fun pc _ => term_val ty.unit pc
+      (* | pat_enum E => *)
+      (*     fun v _ => term_val (ty.enum E) v *)
+      | pat_bvec_split m n x y =>
+          fun _ Exy =>
+            let (Ex,vr) := env.view Exy in
+            let (E,vl)  := env.view Ex in
+            term_binop bop.bvapp vl vr
+      (* | pat_bvec_exhaustive m => *)
+      (*     fun v _ => term_val (ty.bvec m) v *)
+      (* | pat_tuple p => *)
+      (*     fun _ ts => term_tuple (tuple_pattern_match_env_reverse p ts) *)
+      (* | pat_record R Δ p => *)
+      (*     fun _ ts => term_record R (record_pattern_match_env_reverse p ts) *)
+      (* | pat_union U x => *)
+      (*     fun '(existT K pc) ts => term_union U K (pattern_match_term_reverse (x K) pc ts) *)
+      end.
 
-  (*   Lemma inst_unfreshen_namedenv (n : N -> LVar) {Σ Σ' Δ} *)
-  (*     (ζ : Sub (freshen_ctx n Σ Δ) Σ') (ι : Valuation Σ') : *)
-  (*     inst (unfreshen_namedenv n ζ) ι = unfreshen_namedenv n (inst ζ ι). *)
-  (*   Proof. induction Δ; cbn in ζ; env.destroy ζ; cbn; f_equal; apply IHΔ. Qed. *)
+    (* Lemma inst_pattern_match_term_reverse {Σ σ} (ι : Valuation Σ) (pat : @Pattern N σ) : *)
+    (*   forall (pc : PatternCase pat) (ts : NamedEnv (Term Σ) (PatternCaseCtx pc)), *)
+    (*     inst (pattern_match_term_reverse pat pc ts) ι = *)
+    (*     pattern_match_val_reverse pat pc (inst (T := fun Σ => NamedEnv (Term Σ) _) ts ι). *)
+    (* Proof. *)
+    (*   induction pat; cbn. *)
+    (*   - intros _ ts. now env.destroy ts. *)
+    (*   - reflexivity. *)
+    (*   - intros [] ts. *)
+    (*     + reflexivity. *)
+    (*     + now env.destroy ts. *)
+    (*   - intros _ ts. now env.destroy ts. *)
+    (*   - intros [] ts; now env.destroy ts. *)
+    (*   - intros [] ts. reflexivity. *)
+    (*   - reflexivity. *)
+    (*   - intros _ ts. now env.destroy ts. *)
+    (*   - reflexivity. *)
+    (*   - intros _ ts. *)
+    (*     now rewrite <- inst_tuple_pattern_match_reverse. *)
+    (*   - intros _ ts. f_equal. *)
+    (*     apply inst_record_pattern_match_reverse. *)
+    (*   - intros [] ts. cbn. f_equal. f_equal. apply H. *)
+    (* Qed. *)
 
-  (*   Lemma inst_unfreshen_patterncaseenv (n : N -> LVar) {Σ Σ' σ} (pat : @Pattern N σ) *)
-  (*     (pc : PatternCase (freshen_pattern n Σ pat)) *)
-  (*     (ζ : Sub (PatternCaseCtx pc) Σ') *)
-  (*     (ι : Valuation Σ') : *)
-  (*     inst (unfreshen_patterncaseenv n pat pc ζ) ι = *)
-  (*     unfreshen_patterncaseenv n pat pc (inst ζ ι). *)
-  (*   Proof. *)
-  (*     induction pat; cbn in pc; try destruct pc; cbn in ζ, ι; env.destroy ζ; *)
-  (*       env.destroy ι; cbn; auto using inst_unfreshen_namedenv. *)
-  (*   Qed. *)
+    Lemma inst_unfreshen_namedenv (n : N -> LVar) {Σ Σ' Δ}
+      (ζ : Sub (freshen_ctx n Σ Δ) Σ') (ι : Valuation Σ') :
+      inst (unfreshen_namedenv n ζ) ι = unfreshen_namedenv n (inst ζ ι).
+    Proof. induction Δ; cbn in ζ; env.destroy ζ; cbn; f_equal; apply IHΔ. Qed.
 
-  (* End PatternMatching. *)
+    Lemma inst_unfreshen_patterncaseenv (n : N -> LVar) {Σ Σ' σ} (pat : @Pattern N σ)
+      (pc : PatternCase (freshen_pattern n Σ pat))
+      (ζ : Sub (PatternCaseCtx pc) Σ')
+      (ι : Valuation Σ') :
+      inst (unfreshen_patterncaseenv n pat pc ζ) ι =
+      unfreshen_patterncaseenv n pat pc (inst ζ ι).
+    Proof.
+      induction pat; cbn in pc; try destruct pc; cbn in ζ, ι; env.destroy ζ;
+        env.destroy ι; cbn; auto using inst_unfreshen_namedenv.
+    Qed.
+
+  End PatternMatching.
 
   Import env.notations.
 
